Stubbed out Equiv chapter from Programming Language Foundations

SoftwareFoundations/ProgrammingLanguageFoundations/Equiv.lean
@@ -7,250 +7,905 @@ import Mathlib.tactic.linarith
 import «SoftwareFoundations».«LogicalFoundations».«Maps»
 import «SoftwareFoundations».«LogicalFoundations».«Imp»
 
-/-
-## Behavioral Equivalence
--/
+namespace SoftwareFoundations.ProgrammingLanguageFoundations.Equiv
+  /-
+  ## Behavioral Equivalence
+  -/
 
-/-
-### Definitions
--/
+  /-
+  ### Definitions
+  -/
 
-def Arith.equiv (a₁ a₂: Arith): Prop := ∀ s: State, a₁.eval s = a₂.eval s
-def Logic.equiv (l₁ l₂: Logic): Prop := ∀ s: State, l₁.eval s = l₂.eval s
+  @[reducible] def _root_.Arith.equiv (a₁ a₂: Arith): Prop := ∀ s: State, a₁.eval s = a₂.eval s
+  @[reducible] def _root_.Logic.equiv (l₁ l₂: Logic): Prop := ∀ s: State, l₁.eval s = l₂.eval s
 
-example: (Arith.minus "X" "X").equiv (Arith.num 0) := by
-  unfold Arith.equiv
-  intro s
-  simp
+  @[reducible] def _root_.Command.equiv (c₁ c₂: Command): Prop := ∀ s₁ s₂: State, CommandEval c₁ s₁ s₂ ↔ CommandEval c₂ s₁ s₂
+  @[reducible] def _root_.Command.refines (c₁ c₂: Command): Prop := ∀ s₁ s₂: State, CommandEval c₁ s₁ s₂ → CommandEval c₂ s₁ s₂
 
-example: (Logic.eq (.minus "X" "X") 0).equiv .true := by
-  unfold Logic.equiv
-  intro s
-  simp
-  unfold Arith.eval
-  rfl
+  namespace Term
+    example: (Arith.minus "X" "X").equiv (Arith.num 0) :=
+      fun s =>
+        calc (Arith.minus "X" "X").eval s
+          _ = (s "X") - (s "X")    := rfl
+          _ = 0                    := Nat.sub_self (s "X")
+          _ = (Arith.num 0).eval s := rfl
 
-def Command.equiv (c₁ c₂: Command): Prop := ∀ s₁ s₂: State, CommandEval c₁ s₁ s₂ ↔ CommandEval c₂ s₁ s₂
-def Command.refines (c₁ c₂: Command): Prop := ∀ s₁ s₂: State, CommandEval c₁ s₁ s₂ → CommandEval c₂ s₁ s₂
+    example: (Logic.eq (.minus "X" "X") 0).equiv .true :=
+      fun s =>
+        calc (Logic.eq (.minus "X" "X") 0).eval s
+          _ = BEq.beq ((s "X") - (s "X")) 0 := rfl
+          _ = BEq.beq 0 0                   := congrFun (congrArg BEq.beq (Nat.sub_self (s "X"))) 0
+          _ = .true                         := rfl
+  end Term
 
-/-
-### Simple Examples
--/
+  namespace Tactic
+    example: (Arith.minus "X" "X").equiv (Arith.num 0) := by
+      unfold Arith.equiv
+      intro s
+      simp
 
-example (c: Command): (Command.seq .skip c).equiv c :=
-  fun s₁ s₂ =>
-    have mp: CommandEval (Command.seq .skip c) s₁ s₂ → CommandEval c s₁ s₂
-      | .seq .skip c _ _ s₃ (.skip s) h₂ => h₂
-    have mpr: CommandEval c s₁ s₂ → CommandEval (Command.seq .skip c) s₁ s₂
-      | .skip _                        => .seq _ _ _ _ _ (.skip _) (.skip _)
-      | .assign _ _ _ _ h              => .seq _ _ _ _ _ (.skip _) (.assign _ _ _ _ h)
-      | .seq _ _ _ s₂ _ h₁ h₂          => .seq _ _ _ _ _ (.skip _) (.seq _ _ _ s₂ _ h₁ h₂)
-      | .ifTrue _ _ _ _ _ h₁ h₂        => .seq _ _ _ _ _ (.skip _) (.ifTrue _ _ _ _ _ h₁ h₂)
-      | .ifFalse _ _ _ _ _ h₁ h₂       => .seq _ _ _ _ _ (.skip _) (.ifFalse _ _ _ _ _ h₁ h₂)
-      | .whileTrue _ s₂ _ _ _ h₁ h₂ h₃ => .seq _ _ _ _ _ (.skip _) (.whileTrue _ s₂ _ _ _ h₁ h₂ h₃)
-      | .whileFalse _ _ _ h₁           => .seq _ _ _ _ _ (.skip _) (.whileFalse _ _ _ h₁)
-    ⟨mp, mpr⟩
+    example: (Logic.eq (.minus "X" "X") 0).equiv .true := by
+      unfold Logic.equiv
+      intro s
+      simp
+      unfold Arith.eval
+      rfl
+  end Tactic
 
-theorem Command.skip_left (c: Command): (Command.seq .skip c).equiv c := by
-  unfold Command.equiv
-  intro s₁ s₂
-  apply Iff.intro
-  · intro h
-    cases h with
-      | seq c₁ c₂ s₁ s₂ s₃ h₁ h₂ =>
-        cases h₁ with
-          | skip => exact h₂
-  · intro h
-    cases h
-    <;> try (apply CommandEval.seq
-             · apply CommandEval.skip
-             . constructor
-               repeat assumption)
-    case ifFalse =>
-      apply CommandEval.seq
-      · apply CommandEval.skip
-      . apply CommandEval.ifFalse
-        repeat assumption
-    case whileFalse =>
-      apply CommandEval.seq
-      · apply CommandEval.skip
-      · apply CommandEval.whileFalse
-        repeat assumption
+  namespace Blended
+    example: (Arith.minus "X" "X").equiv (Arith.num 0) :=
+      fun s =>
+        calc (Arith.minus "X" "X").eval s
+          _ = (s "X") - (s "X")    := by rfl
+          _ = 0                    := by rw [Nat.sub_self]
+          _ = (Arith.num 0).eval s := by rfl
 
 
-example (c: Command): (Command.seq c .skip).equiv c :=
-  fun s₁ s₂ =>
-    have mp: CommandEval (Command.seq c .skip) s₁ s₂ → CommandEval c s₁ s₂
-      | .seq c .skip s₁ s _ h₁ (.skip _) => h₁
-    have mpr: CommandEval c s₁ s₂ → CommandEval (Command.seq c .skip) s₁ s₂
-      | .skip _                        => .seq _ _ _ _ _ (.skip _) (.skip _)
-      | .assign _ _ _ _ h              => .seq _ _ _ _ _ (.assign _ _ _ _ h) (.skip _)
-      | .seq _ _ _ s₂ _ h₁ h₂          => .seq _ _ _ _ _ (.seq _ _ _ s₂ _ h₁ h₂) (.skip _)
-      | .ifTrue _ _ _ _ _ h₁ h₂        => .seq _ _ _ _ _ (.ifTrue _ _ _ _ _ h₁ h₂) (.skip _)
-      | .ifFalse _ _ _ _ _ h₁ h₂       => .seq _ _ _ _ _ (.ifFalse _ _ _ _ _ h₁ h₂) (.skip _)
-      | .whileTrue _ s₂ _ _ _ h₁ h₂ h₃ => .seq _ _ _ _ _ (.whileTrue _ s₂ _ _ _ h₁ h₂ h₃) (.skip _)
-      | .whileFalse _ _ _ h₁           => .seq _ _ _ _ _ (.whileFalse _ _ _ h₁) (.skip _)
-    ⟨mp, mpr⟩
+    example: (Logic.eq (.minus "X" "X") 0).equiv .true :=
+      fun s =>
+        calc (Logic.eq (.minus "X" "X") 0).eval s
+          _ = BEq.beq ((s "X") - (s "X")) 0 := by rfl
+          _ = BEq.beq 0 0                   := by rw [Nat.sub_self]
+          _ = .true                         := by rfl
+  end Blended
 
-theorem Command.skip_right (c: Command): (Command.seq c .skip).equiv c := by
-  unfold Command.equiv
-  intro s₁ s₂
-  apply Iff.intro
-  · intro h
-    cases h with
-      | seq c₁ c₂ s₁ s₂ s₃ h₁ h₂ =>
-        cases h₂ with
-          | skip => exact h₁
-  · intro h
-    cases h
-    <;> try (apply CommandEval.seq
-             . constructor
-               repeat assumption
-             · apply CommandEval.skip)
-    case ifFalse =>
-      apply CommandEval.seq
-      . apply CommandEval.ifFalse
-        repeat assumption
-      · apply CommandEval.skip
-    case whileFalse =>
-      apply CommandEval.seq
-      · apply CommandEval.whileFalse
-        repeat assumption
-      · apply CommandEval.skip
+  /-
+  ### Simple Examples
+  -/
 
-example (t f: Command): (Command.if .true t f).equiv t :=
-  fun s₁ s₂ =>
-    have mp: CommandEval (.if .true t f) s₁ s₂ → CommandEval t s₁ s₂
-      | .ifTrue _ _ _ _ _ _ h₂ => h₂
-      | .ifFalse _ _ _ _ _ _ _ => by contradiction -- TODO: Remove the tactic block
-    have mpr: CommandEval t s₁ s₂ → CommandEval (.if .true t f) s₁ s₂
-      | .skip _                        => .ifTrue _ _ _ _ _ rfl (.skip _)
-      | .assign _ _ _ _ h              => .ifTrue _ _ _ _ _ rfl (.assign _ _ _ _ h)
-      | .seq _ _ _ s _ h₁ h₂           => .ifTrue _ _ _ _ _ rfl (.seq _ _ _ s _ h₁ h₂)
-      | .ifTrue _ _ _ _ _ h₁ h₂        => .ifTrue _ _ _ _ _ rfl (.ifTrue _ _ _ _ _ h₁ h₂)
-      | .ifFalse _ _ _ _ _ h₁ h₂       => .ifTrue _ _ _ _ _ rfl (.ifFalse _ _ _ _ _ h₁ h₂)
-      | .whileTrue _ s₂ _ _ _ h₁ h₂ h₃ => .ifTrue _ _ _ _ _ rfl (.whileTrue _ s₂ _ _ _ h₁ h₂ h₃)
-      | .whileFalse _ _ _ h            => .ifTrue _ _ _ _ _ rfl (.whileFalse _ _ _ h)
-    ⟨mp, mpr⟩
+  namespace Term
+    theorem Command.skip_left (c: Command): (Command.seq .skip c).equiv c :=
+      fun s₁ s₂ =>
+        have mp: CommandEval (Command.seq .skip c) s₁ s₂ → CommandEval c s₁ s₂
+          | .seq .skip c _ _ s₃ (.skip s) h₂ => h₂
+        have mpr: CommandEval c s₁ s₂ → CommandEval (Command.seq .skip c) s₁ s₂
+          | .skip _                        => .seq _ _ _ _ _ (.skip _) (.skip _)
+          | .assign _ _ _ _ h              => .seq _ _ _ _ _ (.skip _) (.assign _ _ _ _ h)
+          | .seq _ _ _ s₂ _ h₁ h₂          => .seq _ _ _ _ _ (.skip _) (.seq _ _ _ s₂ _ h₁ h₂)
+          | .ifTrue _ _ _ _ _ h₁ h₂        => .seq _ _ _ _ _ (.skip _) (.ifTrue _ _ _ _ _ h₁ h₂)
+          | .ifFalse _ _ _ _ _ h₁ h₂       => .seq _ _ _ _ _ (.skip _) (.ifFalse _ _ _ _ _ h₁ h₂)
+          | .whileTrue _ s₂ _ _ _ h₁ h₂ h₃ => .seq _ _ _ _ _ (.skip _) (.whileTrue _ s₂ _ _ _ h₁ h₂ h₃)
+          | .whileFalse _ _ _ h₁           => .seq _ _ _ _ _ (.skip _) (.whileFalse _ _ _ h₁)
+        ⟨mp, mpr⟩
 
-theorem Command.if_true_simple (t f: Command): (Command.if .true t f).equiv t := by
-  unfold Command.equiv
-  intro s₁ s₂
-  apply Iff.intro
-  · intro h
-    cases h with
-      | ifTrue _ _ _ _ _ _ h₂ => exact h₂
-      | ifFalse => contradiction
-  · intro h
-    cases h
-    <;> try (apply CommandEval.ifTrue
-             · unfold Logic.eval
-               rfl
-             · constructor
-               repeat assumption)
+    theorem Command.skip_right (c: Command): (Command.seq c .skip).equiv c :=
+      fun s₁ s₂ =>
+        have mp: CommandEval (Command.seq c .skip) s₁ s₂ → CommandEval c s₁ s₂
+          | .seq _ _ _ _ _ h₁ (.skip _) => h₁
+        have mpr: CommandEval c s₁ s₂ → CommandEval (Command.seq c .skip) s₁ s₂
+          | .skip _                        => .seq _ _ _ _ _ (.skip _) (.skip _)
+          | .assign _ _ _ _ h              => .seq _ _ _ _ _ (.assign _ _ _ _ h) (.skip _)
+          | .seq _ _ _ s₂ _ h₁ h₂          => .seq _ _ _ _ _ (.seq _ _ _ s₂ _ h₁ h₂) (.skip _)
+          | .ifTrue _ _ _ _ _ h₁ h₂        => .seq _ _ _ _ _ (.ifTrue _ _ _ _ _ h₁ h₂) (.skip _)
+          | .ifFalse _ _ _ _ _ h₁ h₂       => .seq _ _ _ _ _ (.ifFalse _ _ _ _ _ h₁ h₂) (.skip _)
+          | .whileTrue _ s₂ _ _ _ h₁ h₂ h₃ => .seq _ _ _ _ _ (.whileTrue _ s₂ _ _ _ h₁ h₂ h₃) (.skip _)
+          | .whileFalse _ _ _ h₁           => .seq _ _ _ _ _ (.whileFalse _ _ _ h₁) (.skip _)
+        ⟨mp, mpr⟩
 
-    case ifFalse c t f h₁ h₂ =>
-      apply CommandEval.ifTrue
-      · unfold Logic.eval
-        rfl
-      . constructor
-        · sorry
-        · sorry
-    case whileFalse c b h₁ =>
-      apply CommandEval.ifTrue
-      · unfold Logic.eval
-        rfl
-      . constructor
-        · sorry
-        · sorry
-        · sorry
-        · sorry
+    example (t f: Command): (Command.if .true t f).equiv t :=
+      fun s₁ s₂ =>
+        have mp: CommandEval (.if .true t f) s₁ s₂ → CommandEval t s₁ s₂
+          | .ifTrue _ _ _ _ _ _ h₂ => h₂
+          | .ifFalse _ _ _ _ _ _ _ => by contradiction -- TODO: Remove the tactic block
+        have mpr: CommandEval t s₁ s₂ → CommandEval (.if .true t f) s₁ s₂
+          | .skip _                        => .ifTrue _ _ _ _ _ rfl (.skip _)
+          | .assign _ _ _ _ h              => .ifTrue _ _ _ _ _ rfl (.assign _ _ _ _ h)
+          | .seq _ _ _ s _ h₁ h₂           => .ifTrue _ _ _ _ _ rfl (.seq _ _ _ s _ h₁ h₂)
+          | .ifTrue _ _ _ _ _ h₁ h₂        => .ifTrue _ _ _ _ _ rfl (.ifTrue _ _ _ _ _ h₁ h₂)
+          | .ifFalse _ _ _ _ _ h₁ h₂       => .ifTrue _ _ _ _ _ rfl (.ifFalse _ _ _ _ _ h₁ h₂)
+          | .whileTrue _ s₂ _ _ _ h₁ h₂ h₃ => .ifTrue _ _ _ _ _ rfl (.whileTrue _ s₂ _ _ _ h₁ h₂ h₃)
+          | .whileFalse _ _ _ h            => .ifTrue _ _ _ _ _ rfl (.whileFalse _ _ _ h)
+        ⟨mp, mpr⟩
 
-example (b: Logic) (c₁ c₂: Command) (h₁: b.equiv .true): (Command.if b c₁ c₂).equiv c₁ := by sorry
-theorem Command.if_true (b: Logic) (c₁ c₂: Command) (h₁: b.equiv .true): (Command.if b c₁ c₂).equiv c₁ := by sorry
+    theorem Command.if_true (b: Logic) (c₁ c₂: Command) (h: b.equiv .true): (Command.if b c₁ c₂).equiv c₁ :=
+      fun s₁ s₂ =>
+        -- TODO: Remove tactic block
+        have hₑ: b.eval s₁ = .true := by simp_all
+        have mp: CommandEval (.if b c₁ c₂) s₁ s₂ → CommandEval c₁ s₁ s₂
+          | .ifTrue _ _ _ _ _ _ h₂ => h₂
+          | .ifFalse _ _ _ _ _ h₁ _ =>
+            have h₅: false = true :=
+              calc false
+                _ = b.eval s₁           := Eq.symm h₁
+                _ = Logic.eval s₁ .true := h s₁
+                _ = true                := rfl
+            by contradiction -- TODO: Remove tactic block
+        have mpr: CommandEval c₁ s₁ s₂ → CommandEval (.if b c₁ c₂) s₁ s₂
+          | .skip _                       => .ifTrue _ _ _ _ _ hₑ (.skip _)
+          | .assign _ _ _ _ h₁            => .ifTrue _ _ _ _ _ hₑ (.assign _ _ _ _ h₁)
+          | .seq _ _ _ _ _ h₁ h₂          => .ifTrue _ _ _ _ _ hₑ (.seq _ _ _ _ _ h₁ h₂)
+          | .ifTrue _ _ _ _ _ h₁ h₂       => .ifTrue _ _ _ _ _ hₑ (.ifTrue _ _ _ _ _ h₁ h₂)
+          | .ifFalse _ _ _ _ _ h₁ h₂      => .ifTrue _ _ _ _ _ hₑ (.ifFalse _ _ _ _ _ h₁ h₂)
+          | .whileTrue _ _ _ _ _ h₁ h₂ h₃ => .ifTrue _ _ _ _ _ hₑ (.whileTrue _ _ _ _ _ h₁ h₂ h₃)
+          | .whileFalse _ _ _ h₁          => .ifTrue _ _ _ _ _ hₑ (.whileFalse _ _ _ h₁)
+        ⟨mp, mpr⟩
 
-example (b: Logic) (c₁ c₂: Command) (h₁: b.equiv .false): (Command.if b c₁ c₂).equiv c₂ := by sorry
-theorem Command.if_false (b: Logic) (c₁ c₂: Command) (h₁: b.equiv .false): (Command.if b c₁ c₂).equiv c₂ := by sorry
+    theorem Command.if_false (b: Logic) (c₁ c₂: Command) (h₁: b.equiv .false): (Command.if b c₁ c₂).equiv c₂ :=
+      fun s₁ s₂ =>
+        have hₑ: b.eval s₁ = .false := by simp_all
+        have mp: CommandEval (.if b c₁ c₂) s₁ s₂ → CommandEval c₂ s₁ s₂ := sorry
+        have mpr: CommandEval c₂ s₁ s₂ → CommandEval (.if b c₁ c₂) s₁ s₂ := sorry
+        ⟨mp, mpr⟩
 
-example (b: Logic) (c₁ c₂: Command): (Command.if b c₁ c₂).equiv (Command.if (.not b) c₂ c₁) := sorry
-theorem Command.if_swap (b: Logic) (c₁ c₂: Command): (Command.if b c₁ c₂).equiv (Command.if (.not b) c₂ c₁) := by sorry
+    theorem Command.if_swap (b: Logic) (c₁ c₂: Command): (Command.if b c₁ c₂).equiv (Command.if (.not b) c₂ c₁) :=
+      fun s₁ s₂ =>
+        have mp: CommandEval (.if b c₁ c₂) s₁ s₂ → CommandEval (.if (.not b) c₂ c₁) s₁ s₂ := sorry
+        have mpr: CommandEval (.if (.not b) c₂ c₁) s₁ s₂ → CommandEval (.if b c₁ c₂) s₁ s₂ := sorry
+        ⟨mp, mpr⟩
 
-example (c: Logic) (b: Command) (h₁: c.equiv .false): (Command.while c b).equiv Command.skip :=
-  sorry
-  where
-    while_false_nonterm: Nat := sorry
-theorem Command.while_false (c: Logic) (b: Command) (h₁: c.equiv .false): (Command.while c b).equiv Command.skip := by
-  sorry
-  where
-    while_false_nonterm: Nat := sorry
+    theorem Command.while_false (c: Logic) (b: Command) (h₁: c.equiv .false): (Command.while c b).equiv Command.skip :=
+      fun s₁ s₂ =>
+        have hₑ: c.eval s₁ = .false := by simp_all
+        have mp: CommandEval (.while c b) s₁ s₂ → CommandEval .skip s₁ s₂ := sorry
+        have mpr: CommandEval .skip s₁ s₂ → CommandEval (.while c b) s₁ s₂ := sorry
+        ⟨mp, mpr⟩
+      where
+        nonterm: Nat := sorry
 
-example (c: Logic) (b: Command) (h₁: c.equiv .true): (Command.while c b).equiv (Command.while .true Command.skip) :=
-  sorry
-  where
-    while_true_nonterm: Nat := sorry
-theorem Command.while_true (c: Logic) (b: Command) (h₁: c.equiv .true): (Command.while c b).equiv (Command.while .true Command.skip) := by
-  sorry
-  where
-    while_true_nonterm: Nat := sorry
+    theorem Command.while_true (c: Logic) (b: Command) (h₁: c.equiv .true): (Command.while c b).equiv (Command.while .true Command.skip) :=
+      fun s₁ s₂ =>
+        have hₑ: c.eval s₁ = .true := by simp_all
+        have mp: CommandEval (.while c b) s₁ s₂ → CommandEval (.while .true .skip) s₁ s₂ := sorry
+        have mpr: CommandEval (.while .true .skip) s₁ s₂ → CommandEval (.while c b) s₁ s₂ := sorry
+        ⟨mp, mpr⟩
+      where
+        nonterm: Nat := sorry
 
-example (c: Logic) (b: Command): (Command.while c b).equiv (Command.if c (Command.seq b (Command.while c b)) .skip) := sorry
-theorem Command.loop_unrolling (c: Logic) (b: Command): (Command.while c b).equiv (Command.if c (Command.seq b (Command.while c b)) .skip) := by sorry
+    theorem Command.loop_unrolling (c: Logic) (b: Command): (Command.while c b).equiv (Command.if c (Command.seq b (Command.while c b)) .skip) :=
+      fun s₁ s₂ =>
+        have mp: CommandEval (.while c b) s₁ s₂ → CommandEval (.if c (.seq b (.while c b)) .skip) s₁ s₂ := sorry
+        have mpr: CommandEval (.if c (.seq b (.while c b)) .skip) s₁ s₂ → CommandEval (.while c b) s₁ s₂ := sorry
+        ⟨mp, mpr⟩
 
-example (c₁ c₂ c₂: Command): (Command.seq (Command.seq c₁ c₂) c₃).equiv (Command.seq c₁ (Command.seq c₂ c₃)) := sorry
-theorem Command.seq_assoc (c₁ c₂ c₂: Command): (Command.seq (Command.seq c₁ c₂) c₃).equiv (Command.seq c₁ (Command.seq c₂ c₃)) := by sorry
+    theorem Command.seq_assoc (c₁ c₂ c₂: Command): (Command.seq (Command.seq c₁ c₂) c₃).equiv (Command.seq c₁ (Command.seq c₂ c₃)) :=
+      fun s₁ s₂ =>
+        have mp: CommandEval (.seq (.seq c₁ c₂) c₃) s₁ s₂ → CommandEval (.seq c₁ (.seq c₂ c₃)) s₁ s₂ := sorry
+        have mpr: CommandEval (.seq c₁ (.seq c₂ c₃)) s₁ s₂ → CommandEval (.seq (.seq c₁ c₂) c₃) s₁ s₂ := sorry
+        ⟨mp, mpr⟩
 
-example (id: String): (Command.assign "X" "X").equiv Command.skip := sorry
-theorem Command.identity_assignment (id: String): (Command.assign "X" "X").equiv Command.skip := by sorry
+    theorem Command.identity_assignment (id: String): (Command.assign id id).equiv Command.skip :=
+      fun s₁ s₂ =>
+        have mp: CommandEval (.assign id id) s₁ s₂ → CommandEval .skip s₁ s₂ := sorry
+        have mpr: CommandEval .skip s₁ s₂ → CommandEval (.assign id id) s₁ s₂ := sorry
+        ⟨mp, mpr⟩
 
-example (id: String) (e: Arith) (h₁: (id: Arith).equiv e): Command.skip.equiv (Command.assign id e) := sorry
-theorem Command.assign_arith_equiv (id: String) (e: Arith) (h₁: (id: Arith).equiv e): Command.skip.equiv (Command.assign id e) := by sorry
+    theorem Command.assign_arith_equiv (id: String) (e: Arith) (h: (id: Arith).equiv e): Command.skip.equiv (Command.assign id e) :=
+      fun s₁ s₂ =>
+        have mp: CommandEval .skip s₁ s₂ → CommandEval (.assign id e) s₁ s₂ := sorry
+        have mpr: CommandEval (.assign id e) s₁ s₂ → CommandEval .skip s₁ s₂ := sorry
+        ⟨mp, mpr⟩
+  end Term
 
-section
-  private def a: Command :=
-    .while (.gt "X" 0)
-      (.assign "X" ("X" + 1))
+  namespace Tactic
+    theorem Command.skip_left (c: Command): (Command.seq .skip c).equiv c := by
+      unfold Command.equiv
+      intro s₁ s₂
+      apply Iff.intro
+      · intro h
+        cases h with
+          | seq c₁ c₂ s₁ s₂ s₃ h₁ h₂ =>
+            cases h₁ with
+              | skip => exact h₂
+      · intro h
+        cases h
+        <;> try (apply CommandEval.seq
+                 · apply CommandEval.skip
+                 . constructor
+                   repeat assumption)
+        case ifFalse =>
+          apply CommandEval.seq
+          · apply CommandEval.skip
+          . apply CommandEval.ifFalse
+            repeat assumption
+        case whileFalse =>
+          apply CommandEval.seq
+          · apply CommandEval.skip
+          · apply CommandEval.whileFalse
+            repeat assumption
 
-  private def b: Command :=
-    .seq
-      (.if (.eq "X" 0)
+    theorem Command.skip_right (c: Command): (Command.seq c .skip).equiv c := by
+      unfold Command.equiv
+      intro s₁ s₂
+      apply Iff.intro
+      · intro h
+        cases h with
+          | seq c₁ c₂ s₁ s₂ s₃ h₁ h₂ =>
+            cases h₂ with
+              | skip => exact h₁
+      · intro h
+        cases h
+        <;> try (apply CommandEval.seq
+                 . constructor
+                   repeat assumption
+                 · apply CommandEval.skip)
+        case ifFalse =>
+          apply CommandEval.seq
+          . apply CommandEval.ifFalse
+            repeat assumption
+          · apply CommandEval.skip
+        case whileFalse =>
+          apply CommandEval.seq
+          · apply CommandEval.whileFalse
+            repeat assumption
+          · apply CommandEval.skip
+
+    example (t f: Command): (Command.if .true t f).equiv t := by
+      unfold Command.equiv
+      intro s₁ s₂
+      apply Iff.intro
+      · intro h
+        cases h with
+          | ifTrue _ _ _ _ _ _ h₂ => exact h₂
+          | ifFalse => contradiction
+      · intro h
+        cases h
+        <;> try (apply CommandEval.ifTrue
+                 · unfold Logic.eval
+                   rfl
+                 · constructor
+                   repeat assumption)
+        case ifFalse c t f h₁ h₂ =>
+          apply CommandEval.ifTrue
+          · unfold Logic.eval
+            rfl
+          . apply CommandEval.ifFalse
+            repeat assumption
+        case whileFalse c b h₁ =>
+          apply CommandEval.ifTrue
+          · unfold Logic.eval
+            rfl
+          . apply CommandEval.whileFalse
+            repeat assumption
+
+    theorem Command.if_true (b: Logic) (c₁ c₂: Command) (h₁: b.equiv .true): (Command.if b c₁ c₂).equiv c₁ := by
+      unfold Command.equiv
+      intro s₁ s₂
+      apply Iff.intro
+      · intro h
+        cases h with
+          | ifTrue _ _ _ _ _ _ h₂ => exact h₂
+          | ifFalse _ _ _ _ _ h₃ _ =>
+            unfold Logic.equiv at h₁
+            have h₄ := h₁ s₁
+            rw [h₄] at h₃
+            contradiction
+      · intro h
+        cases h
+        <;> try (apply CommandEval.ifTrue
+                 · unfold Logic.equiv at h₁
+                   apply h₁
+                 · constructor
+                   repeat assumption)
+        case ifFalse =>
+          apply CommandEval.ifTrue
+          · unfold Logic.equiv at h₁
+            apply h₁
+          · apply CommandEval.ifFalse
+            repeat assumption
+        case whileFalse =>
+          apply CommandEval.ifTrue
+          · unfold Logic.equiv at h₁
+            apply h₁
+          · apply CommandEval.whileFalse
+            repeat assumption
+
+    theorem Command.if_false (b: Logic) (c₁ c₂: Command) (h₁: b.equiv .false): (Command.if b c₁ c₂).equiv c₂ := by
+      unfold Command.equiv
+      intro s₁ s₂
+      apply Iff.intro
+      · sorry
+      · sorry
+
+    theorem Command.if_swap (b: Logic) (c₁ c₂: Command): (Command.if b c₁ c₂).equiv (Command.if (.not b) c₂ c₁) := by
+      unfold Command.equiv
+      intro s₁ s₂
+      apply Iff.intro
+      · sorry
+      · sorry
+
+    theorem Command.while_false (c: Logic) (b: Command) (h₁: c.equiv .false): (Command.while c b).equiv Command.skip := by
+      unfold Command.equiv
+      intro s₁ s₂
+      apply Iff.intro
+      · sorry
+      · sorry
+      where
+        nonterm: Nat := sorry
+
+    theorem Command.while_true (c: Logic) (b: Command) (h₁: c.equiv .true): (Command.while c b).equiv (Command.while .true Command.skip) := by
+      unfold Command.equiv
+      intro s₁ s₂
+      apply Iff.intro
+      · sorry
+      · sorry
+      where
+        nonterm: Nat := sorry
+
+    theorem Command.loop_unrolling (c: Logic) (b: Command): (Command.while c b).equiv (Command.if c (Command.seq b (Command.while c b)) .skip) := by
+      unfold Command.equiv
+      intro s₁ s₂
+      apply Iff.intro
+      · sorry
+      · sorry
+
+    theorem Command.seq_assoc (c₁ c₂ c₂: Command): (Command.seq (Command.seq c₁ c₂) c₃).equiv (Command.seq c₁ (Command.seq c₂ c₃)) := by
+      unfold Command.equiv
+      intro s₁ s₂
+      apply Iff.intro
+      · sorry
+      · sorry
+
+    theorem Command.identity_assignment (id: String): (Command.assign "X" "X").equiv Command.skip := by
+      unfold Command.equiv
+      intro s₁ s₂
+      apply Iff.intro
+      · sorry
+      · sorry
+
+    theorem Command.assign_arith_equiv (id: String) (e: Arith) (h₁: (id: Arith).equiv e): Command.skip.equiv (Command.assign id e) := by
+      unfold Command.equiv
+      intro s₁ s₂
+      apply Iff.intro
+      · sorry
+      · sorry
+  end Tactic
+
+  namespace Blended
+    theorem Command.skip_left (c: Command): (Command.seq .skip c).equiv c := by sorry
+    theorem Command.skip_right (c: Command): (Command.seq c .skip).equiv c := by sorry
+    example (t f: Command): (Command.if .true t f).equiv t := by sorry
+    theorem Command.if_true (b: Logic) (c₁ c₂: Command) (h₁: b.equiv .true): (Command.if b c₁ c₂).equiv c₁ := by sorry
+    theorem Command.if_false (b: Logic) (c₁ c₂: Command) (h₁: b.equiv .false): (Command.if b c₁ c₂).equiv c₂ := by sorry
+    theorem Command.if_swap (b: Logic) (c₁ c₂: Command): (Command.if b c₁ c₂).equiv (Command.if (.not b) c₂ c₁) := by sorry
+    theorem Command.while_false (c: Logic) (b: Command) (h₁: c.equiv .false): (Command.while c b).equiv Command.skip := by sorry
+    theorem Command.while_true (c: Logic) (b: Command) (h₁: c.equiv .true): (Command.while c b).equiv (Command.while .true Command.skip) := by sorry
+    theorem Command.loop_unrolling (c: Logic) (b: Command): (Command.while c b).equiv (Command.if c (Command.seq b (Command.while c b)) .skip) := by sorry
+    theorem Command.seq_assoc (c₁ c₂ c₂: Command): (Command.seq (Command.seq c₁ c₂) c₃).equiv (Command.seq c₁ (Command.seq c₂ c₃)) := by sorry
+    theorem Command.identity_assignment (id: String): (Command.assign "X" "X").equiv Command.skip := by sorry
+    theorem Command.assign_arith_equiv (id: String) (e: Arith) (h₁: (id: Arith).equiv e): Command.skip.equiv (Command.assign id e) := by sorry
+  end Blended
+
+  section
+    private def a: Command :=
+      .while (.gt "X" 0)
+        (.assign "X" ("X" + 1))
+
+    private def b: Command :=
+      .seq
+        (.if (.eq "X" 0)
+          (.seq
+            (.assign "X" ("X" + 1))
+            (.assign "Y" 1))
+          (.assign "Y" 0))
         (.seq
-          (.assign "X" ("X" + 1))
-          (.assign "Y" 1))
-        (.assign "Y" 0))
-      (.seq
-        (.assign "X" ("X" - "Y"))
-        (.assign "Y" 0))
+          (.assign "X" ("X" - "Y"))
+          (.assign "Y" 0))
 
-  private def c: Command :=
-    .skip
+    private def c: Command :=
+      .skip
 
-  private def d: Command :=
-    .while (.neq "X" 0)
-      (.assign "X" ("X" * "Y" + 1))
+    private def d: Command :=
+      .while (.neq "X" 0)
+        (.assign "X" ("X" * "Y" + 1))
 
-  private def e: Command :=
-    .assign "Y" 0
+    private def e: Command :=
+      .assign "Y" 0
 
-  private def f: Command :=
+    private def f: Command :=
+      .seq
+        (.assign "Y" ("X" + 1))
+        (.while (.neq "X" "Y")
+          (.assign "Y" ("X" + 1)))
+
+    private def g: Command :=
+      .while .true .skip
+
+    private def h: Command :=
+      .while (.neq "X" "X")
+        (.assign "X" ("X" + 1))
+
+    private def i: Command :=
+      .while (.neq "X" "Y")
+        (.assign "X" ("Y" + 1))
+
+    private def equiv_classes: List (List Command) := []
+  end
+
+  /-
+  ## Properties of Behavioral Equivalence
+  -/
+
+  /-
+  ### Behavioral Equivalence is an Equivalence
+  -/
+
+  namespace Term
+    theorem Arith.equiv.refl (e: Arith): e.equiv e := sorry
+    theorem Arith.equiv.symm (e₁ e₂: Arith) (h: e₁.equiv e₁): e₂.equiv e₁ := sorry
+    theorem Arith.equiv.trans (e₁ e₂ e₃: Arith) (h₁: e₁.equiv e₂) (h₂: e₂.equiv e₃): e₁.equiv e₃ := sorry
+
+    theorem Logic.equiv.refl (b: Logic): b.equiv b := sorry
+    theorem Logic.equiv.symm (b₁ b₂: Logic) (h: b₁.equiv b₂): b₂.equiv b₁ := sorry
+    theorem Logic.equiv.trans (b₁ b₂ b₃: Logic) (h₁: b₁.equiv b₂) (h₂: b₂.equiv b₃): b₁.equiv b₃ := sorry
+
+    theorem Command.equiv.refl (c: Command): c.equiv c := sorry
+    theorem Command.equiv.symm (c₁ c₂: Command) (h: c₁.equiv c₂): c₂.equiv c₁ := sorry
+    theorem Command.equiv.trans (c₁ c₂ c₃: Command) (h₁: c₁.equiv c₂) (h₂: c₂.equiv c₃): c₁.equiv c₃ := sorry
+  end Term
+
+  namespace Tactic
+    theorem Arith.equiv.refl (e: Arith): e.equiv e := by sorry
+    theorem Arith.equiv.symm (e₁ e₂: Arith) (h: e₁.equiv e₁): e₂.equiv e₁ := by sorry
+    theorem Arith.equiv.trans (e₁ e₂ e₃: Arith) (h₁: e₁.equiv e₂) (h₂: e₂.equiv e₃): e₁.equiv e₃ := by sorry
+
+    theorem Logic.equiv.refl (b: Logic): b.equiv b := by sorry
+    theorem Logic.equiv.symm (b₁ b₂: Logic) (h: b₁.equiv b₂): b₂.equiv b₁ := by sorry
+    theorem Logic.equiv.trans (b₁ b₂ b₃: Logic) (h₁: b₁.equiv b₂) (h₂: b₂.equiv b₃): b₁.equiv b₃ := by sorry
+
+    theorem Command.equiv.refl (c: Command): c.equiv c := by sorry
+    theorem Command.equiv.symm (c₁ c₂: Command) (h: c₁.equiv c₂): c₂.equiv c₁ := by sorry
+    theorem Command.equiv.trans (c₁ c₂ c₃: Command) (h₁: c₁.equiv c₂) (h₂: c₂.equiv c₃): c₁.equiv c₃ := by sorry
+  end Tactic
+
+  namespace Blended
+    theorem Arith.equiv.refl (e: Arith): e.equiv e := sorry
+    theorem Arith.equiv.symm (e₁ e₂: Arith) (h: e₁.equiv e₁): e₂.equiv e₁ := sorry
+    theorem Arith.equiv.trans (e₁ e₂ e₃: Arith) (h₁: e₁.equiv e₂) (h₂: e₂.equiv e₃): e₁.equiv e₃ := sorry
+
+    theorem Logic.equiv.refl (b: Logic): b.equiv b := sorry
+    theorem Logic.equiv.symm (b₁ b₂: Logic) (h: b₁.equiv b₂): b₂.equiv b₁ := sorry
+    theorem Logic.equiv.trans (b₁ b₂ b₃: Logic) (h₁: b₁.equiv b₂) (h₂: b₂.equiv b₃): b₁.equiv b₃ := sorry
+
+    theorem Command.equiv.refl (c: Command): c.equiv c := sorry
+    theorem Command.equiv.symm (c₁ c₂: Command) (h: c₁.equiv c₂): c₂.equiv c₁ := sorry
+    theorem Command.equiv.trans (c₁ c₂ c₃: Command) (h₁: c₁.equiv c₂) (h₂: c₂.equiv c₃): c₁.equiv c₃ := sorry
+  end Blended
+
+  /-
+  ### Behavioral Equivalence is a Congruence
+  -/
+
+  private def congr_prog₁: Command :=
     .seq
-      (.assign "Y" ("X" + 1))
-      (.while (.neq "X" "Y")
-        (.assign "Y" ("X" + 1)))
+      (.assign "X" 0)
+      (.if (.eq "X" 0)
+        (.assign "Y" 0)
+        (.assign "Y" 42))
+  private def congr_prog₂: Command :=
+    .seq
+      (.assign "X" 0)
+      (.if (.eq "X" 0)
+        (.assign "Y" ("X" - "X"))
+        (.assign "Y" 42))
 
-  private def g: Command :=
-    .while .true .skip
+  namespace Term
+    theorem Command.skip.congr: Command.skip.equiv .skip := sorry
+    theorem Command.assign.congr (id: String) (e₁ e₂: Arith) (h: e₁.equiv e₂): (Command.assign id e₁).equiv (.assign id e₂) := sorry
+    theorem Command.seq.congr (c₁ c₂ c₃ c₄: Command) (h₁: c₁.equiv c₃) (h₂: c₂.equiv c₄): (Command.seq c₁ c₃).equiv (.seq c₂ c₄) := sorry
+    theorem Command.if.congr (c₁ c₂: Logic) (t₁ t₂ f₁ f₂: Command) (h₁: c₁.equiv c₂) (h₂: t₁.equiv t₂) (h₃: f₁.equiv f₁): (Command.if c₁ t₁ f₁).equiv (.if c₂ t₂ f₂) := sorry
 
-  private def h: Command :=
-    .while (.neq "X" "X")
-      (.assign "X" ("X" + 1))
+    example: congr_prog₁.equiv congr_prog₂ := sorry
+  end Term
 
-  private def i: Command :=
-    .while (.neq "X" "Y")
-      (.assign "X" ("Y" + 1))
+  namespace Tactic
+    theorem Command.skip.congr: Command.skip.equiv .skip := by sorry
+    theorem Command.assign.congr (id: String) (e₁ e₂: Arith) (h: e₁.equiv e₂): (Command.assign id e₁).equiv (.assign id e₂) := by sorry
+    theorem Command.seq.congr (c₁ c₂ c₃ c₄: Command) (h₁: c₁.equiv c₃) (h₂: c₂.equiv c₄): (Command.seq c₁ c₃).equiv (.seq c₂ c₄) := by sorry
+    theorem Command.if.congr (c₁ c₂: Logic) (t₁ t₂ f₁ f₂: Command) (h₁: c₁.equiv c₂) (h₂: t₁.equiv t₂) (h₃: f₁.equiv f₁): (Command.if c₁ t₁ f₁).equiv (.if c₂ t₂ f₂) := by sorry
 
-  private def equiv_classes: List (List Command) := []
-end
+    example: congr_prog₁.equiv congr_prog₂ := by sorry
+  end Tactic
 
-/-
-## Properties of Behavioral Equivalence
--/
+  namespace Blended
+    theorem Command.skip.congr: Command.skip.equiv .skip := sorry
+    theorem Command.assign.congr (id: String) (e₁ e₂: Arith) (h: e₁.equiv e₂): (Command.assign id e₁).equiv (.assign id e₂) := sorry
+    theorem Command.seq.congr (c₁ c₂ c₃ c₄: Command) (h₁: c₁.equiv c₃) (h₂: c₂.equiv c₄): (Command.seq c₁ c₃).equiv (.seq c₂ c₄) := sorry
+    theorem Command.if.congr (c₁ c₂: Logic) (t₁ t₂ f₁ f₂: Command) (h₁: c₁.equiv c₂) (h₂: t₁.equiv t₂) (h₃: f₁.equiv f₁): (Command.if c₁ t₁ f₁).equiv (.if c₂ t₂ f₂) := sorry
+
+    example: congr_prog₁.equiv congr_prog₂ := sorry
+  end Blended
+
+  /-
+  ## Program Transformations
+  -/
+
+  def Arith.trans_sound (t: Arith → Arith): Prop := ∀ e: Arith, e.equiv (t e)
+  def Logic.trans_sound (t: Logic → Logic): Prop := ∀ b: Logic, b.equiv (t b)
+  def Command.trans_sound (t: Command → Command): Prop := ∀ c: Command, c.equiv (t c)
+
+  /-
+  ### Constant Folding Optimization
+  -/
+
+  def _root_.Arith.constFold: _root_.Arith → _root_.Arith
+    | .num n => .num n
+    | .ident id => .ident id
+    | .plus e₁ e₂ =>
+      match constFold e₁, constFold e₂ with
+        | .num n₁, .num n₂ => .num (n₁ + n₂)
+        | e₁, e₂ => .plus e₁ e₂
+    | .minus e₁ e₂ =>
+      match constFold e₁, constFold e₂ with
+        | .num n₁, .num n₂ => .num (n₁ - n₂)
+        | e₁, e₂ => .minus e₁ e₂
+    | .mult e₁ e₂ =>
+      match constFold e₁, constFold e₂ with
+        | .num n₁, .num n₂ => .num (n₁ * n₂)
+        | e₁, e₂ => .mult e₁ e₂
+
+  example: (((1: Arith) + 2) * "X").constFold = 3 * "X" := rfl
+  example: ("X" - (((0: Arith) * 6) + "Y")).constFold = "X" - (0 + "Y") := rfl
+
+  def _root_.Logic.constFold: _root_.Logic → _root_.Logic
+    | .true => .true
+    | .false => .false
+    | .eq e₁ e₂ =>
+      match e₁.constFold, e₂.constFold with
+        | .num n₁, .num n₂ => if n₁ == n₂ then .true else .false
+        | e₁, e₂ => .eq e₁ e₂
+    | .neq e₁ e₂ =>
+      match e₁.constFold, e₂.constFold with
+        | .num n₁, .num n₂ => if n₁ != n₂ then .true else .false
+        | e₁, e₂ => .eq e₁ e₂
+    | .le e₁ e₂ =>
+      match e₁.constFold, e₂.constFold with
+        | .num n₁, .num n₂ => if n₁ ≤ n₂ then .true else .false
+        | e₁, e₂ => .eq e₁ e₂
+    | .gt e₁ e₂ =>
+      match e₁.constFold, e₂.constFold with
+        | .num n₁, .num n₂ => if n₁ > n₂ then .true else .false
+        | e₁, e₂ => .eq e₁ e₂
+    | .not b =>
+      match constFold b with
+        | .true => .false
+        | .false => .true
+        | b => .not b
+    | .and b₁ b₂ =>
+      match constFold b₁, constFold b₂ with
+        -- Note: Avoiding the short-circuiting `_, .false` and `.false, _` cases
+        -- as that can change the termination properties of the `Imp` program.
+        | .true, .true => .true
+        | .true, .false => .false
+        | .false, .true => .false
+        | .false, .false => .false
+        | b₁, b₂ => .and b₁ b₂
+
+  example: (Logic.and .true (.not (.false && .true))).constFold = .true := rfl
+  example: (Logic.and (.eq "X" "Y") (.eq 0 (2 - (1 + 1)))).constFold = .and (.eq "X" "Y") .true := rfl
+
+  def _root_.Command.constFold: Command → Command
+    | .skip => .skip
+    | .assign id e => .assign id e.constFold
+    | .seq c₁ c₂ => .seq c₁.constFold c₂.constFold
+    | .if c t f =>
+      let t: Command := t.constFold
+      let f: Command := f.constFold
+      match c.constFold with
+        | .true => t
+        | .false => f
+        | c => .if c t f
+    | .while c b =>
+      let b: Command := b.constFold
+      match c.constFold with
+        | .true => .while .true .skip
+        | .false => .skip
+        | c => .while c b
+
+  example:
+    (Command.seq
+      (.assign "X" (4 + 5))
+      (Command.seq
+        (.assign "Y" ("X" - 3))
+        (Command.seq
+          (.if (.eq ("X" - "Y") (2 + 4))
+            .skip
+            (.assign "Y" 0))
+          (Command.seq
+            (.if (.le 0 (4 - (2 + 1)))
+              (.assign "Y" 0)
+              .skip)
+            (.while (.eq "Y" 0)
+              (.assign "X" ("X" + 1))))))).constFold
+    =
+    Command.seq
+    (.assign "X" 9)
+    (Command.seq
+      (.assign "Y" ("X" - 3))
+      (Command.seq
+        (.if (.eq ("X" - "Y") 6)
+          .skip
+          (.assign "Y" 0))
+        (Command.seq
+          (.assign "Y" 0)
+          (.while (.eq "Y" 0)
+            (.assign "X" ("X" + 1))))))
+    := rfl
+
+  /-
+  ### Soundness of Constant Folding
+  -/
+
+  namespace Term
+    theorem Arith.constFold.sound: Arith.trans_sound Arith.constFold := sorry
+    theorem Logic.constFold.sound: Logic.trans_sound Logic.constFold := sorry
+    theorem Command.constFold.sound: Command.trans_sound Command.constFold := sorry
+  end Term
+
+  namespace Tactic
+    theorem Arith.constFold.sound: Arith.trans_sound Arith.constFold := by sorry
+    theorem Logic.constFold.sound: Logic.trans_sound Logic.constFold := by sorry
+    theorem Command.constFold.sound: Command.trans_sound Command.constFold := by sorry
+  end Tactic
+
+  namespace Blended
+    theorem Arith.constFold.sound: Arith.trans_sound Arith.constFold := sorry
+    theorem Logic.constFold.sound: Logic.trans_sound Logic.constFold := sorry
+    theorem Command.constFold.sound: Command.trans_sound Command.constFold := sorry
+  end Blended
+
+  /-
+  ### Soundness of `0 + n` Elimination, Redux
+  -/
+
+  def _root_.Arith.opt0Plus: Arith → Arith
+    | .plus (.num 0) e₂ => e₂
+    | e => e
+
+  def _root_.Logic.opt0Plus: Logic → Logic
+    | .eq e₁ e₂ => .eq e₁.opt0Plus e₂.opt0Plus
+    | .neq e₁ e₂ => .neq e₁.opt0Plus e₂.opt0Plus
+    | .le e₁ e₂ => .le e₁.opt0Plus e₂.opt0Plus
+    | .gt e₁ e₂ => .gt e₁.opt0Plus e₂.opt0Plus
+    | .not b => .not (opt0Plus b)
+    | .and b₁ b₂ => .and (opt0Plus b₁) (opt0Plus b₂)
+    | b => b
+
+  def _root_.Command.opt0Plus: Command → Command
+    | .assign id e => .assign id e.opt0Plus
+    | .seq c₁ c₂ => .seq (opt0Plus c₁) (opt0Plus c₂)
+    | .if c t f => .if c.opt0Plus (opt0Plus t) (opt0Plus f)
+    | .while c b => .while c.opt0Plus (opt0Plus b)
+    | c => c
+
+  -- TODO: Fix this
+  -- example: (Command.while (.neq "X" 0) (.assign "X" (0 + "X" - 1))).opt0Plus = .while (.neq "X" 0) (.assign "X" ("X" - 1)) := rfl
+
+  namespace Term
+    theorem Arith.opt0Plus.sound: Arith.trans_sound Arith.opt0Plus := sorry
+    theorem Logic.opt0Plus.sound: Logic.trans_sound Logic.opt0Plus := sorry
+    theorem Command.opt0Plus.sound: Command.trans_sound Command.opt0Plus := sorry
+  end Term
+
+  namespace Tactic
+    theorem Arith.opt0Plus.sound: Arith.trans_sound Arith.opt0Plus := by sorry
+    theorem Logic.opt0Plus.sound: Logic.trans_sound Logic.opt0Plus := by sorry
+    theorem Command.opt0Plus.sound: Command.trans_sound Command.opt0Plus := by sorry
+  end Tactic
+
+  namespace Blended
+    theorem Arith.opt0Plus.sound: Arith.trans_sound Arith.opt0Plus := sorry
+    theorem Logic.opt0Plus.sound: Logic.trans_sound Logic.opt0Plus := sorry
+    theorem Command.opt0Plus.sound: Command.trans_sound Command.opt0Plus := sorry
+  end Blended
+
+  /-
+  #### Transitive Optimization
+  -/
+
+  def Command.opt (c: Command): Command := c.constFold.opt0Plus
+
+  namespace Term
+    theorem Command.opt.sound: Command.trans_sound Command.opt := sorry
+  end Term
+
+  namespace Tactic
+    theorem Command.opt.sound: Command.trans_sound Command.opt := by sorry
+  end Tactic
+
+  namespace Blended
+    theorem Command.opt.sound: Command.trans_sound Command.opt := sorry
+  end Blended
+
+  /-
+  ## Proving Inequivalence
+  -/
+
+  def _root_.Arith.subst (within: Arith) (var: String) (repl: Arith): Arith :=
+    match within with
+      | .num n => .num n
+      | .ident id => if id == var then repl else .ident id
+      | .plus e₁ e₂ => .plus (subst e₁ var repl) (subst e₂ var repl)
+      | .minus e₁ e₂ => .minus (subst e₁ var repl) (subst e₂ var repl)
+      | .mult e₁ e₂ => .mult (subst e₁ var repl) (subst e₂ var repl)
+
+  example: (("Y": Arith) + "X").subst "X" (42 + 53) = "Y" + (42 + 53) := rfl
+
+  def Arith.subst.equiv: Prop := ∀ id₁ id₂ e₁ e₂, (Command.seq (.assign id₁ e₁) (.assign id₂ e₂)).equiv (.seq (.assign id₁ e₁) (.assign id₂ (e₂.subst id₁ e₁)))
+
+  namespace Term
+    theorem Arith.subst.equiv.inequiv: ¬Arith.subst.equiv := sorry
+  end Term
+
+  namespace Tactic
+    theorem Arith.subst.equiv.inequiv: ¬Arith.subst.equiv := by sorry
+  end Tactic
+
+  namespace Blended
+    theorem Arith.subst.equiv.inequiv: ¬Arith.subst.equiv := sorry
+  end Blended
+
+  inductive OccursCheck (var: String): Arith → Prop
+    | num (n: Nat): OccursCheck var (.num n)
+    | ident (id: String) (h: id ≠ var): OccursCheck var (.ident id)
+    | plus (e₁ e₂: Arith) (h₁: OccursCheck var e₁) (h₂: OccursCheck var e₁): OccursCheck var (.plus e₁ e₂)
+    | minus (e₁ e₂: Arith) (h₁: OccursCheck var e₁) (h₂: OccursCheck var e₁): OccursCheck var (.minus e₁ e₂)
+    | mult (e₁ e₂: Arith) (h₁: OccursCheck var e₁) (h₂: OccursCheck var e₁): OccursCheck var (.mult e₁ e₂)
+
+  -- TODO: Weakening Lemma and Proper Substitution Equivalence
+
+  namespace Term
+    example: ¬((Command.while .true .skip).equiv .skip) := sorry
+  end Term
+
+  namespace Tactic
+    example: ¬((Command.while .true .skip).equiv .skip) := by sorry
+  end Tactic
+
+  namespace Blended
+    example: ¬((Command.while .true .skip).equiv .skip) := sorry
+  end Blended
+
+  /-
+  ## Extended Exercise: Nondeterministic Imp
+  -/
+
+  namespace Havoc
+    inductive Command: Type where
+      | skip: Command
+      | assign (id: String) (e: Arith): Command
+      | seq (c₁ c₂: Command): Command
+      | if (b: Logic) (c₁ c₂: Command): Command
+      | while (b: Logic) (c: Command): Command
+      | havoc (id: String): Command
+
+    inductive CommandEval: Command → State → State → Prop where
+      | skip (state: State): CommandEval .skip state state
+      | assign (state: State) (e: Arith) (n: Nat) (id: String) (h: e.eval state = n): CommandEval (.assign id e) state (state.update id n)
+      | seq (c₁ c₂: Command) (s₁ s₂ s₃: State) (h₁: CommandEval c₁ s₁ s₂) (h₂: CommandEval c₂ s₂ s₃): CommandEval (.seq c₁ c₂) s₁ s₃
+      | ifTrue (s₁ s₂: State) (c: Logic) (t f: Command) (h₁: c.eval s₁ = .true) (h₂: CommandEval t s₁ s₂): CommandEval (.if c t f) s₁ s₂
+      | ifFalse (s₁ s₂: State) (c: Logic) (t f: Command) (h₁: c.eval s₁ = .false) (h₂: CommandEval f s₁ s₂): CommandEval (.if c t f) s₁ s₂
+      | whileTrue (s₁ s₂ s₃: State) (c: Logic) (b: Command) (h₁: c.eval s₁ = .true) (h₂: CommandEval b s₁ s₂) (h₃: CommandEval (.while c b) s₂ s₃): CommandEval (.while c b) s₁ s₃
+      | whileFalse (c: Logic) (s: State) (b: Command) (h₁: c.eval s = .false): CommandEval (.while c b) s s
+      -- TODO: Define this properly
+      | havoc (s₁ s₂: State) (id: String): CommandEval (.havoc id) s₁ s₂
+
+    def Command.equiv (c₁ c₂: Command): Prop := ∀ s₁ s₂: State, CommandEval c₁ s₁ s₂ ↔ CommandEval c₂ s₁ s₂
+
+    private def xy: Command := .seq (.havoc "X") (.havoc "Y")
+    private def yx: Command := .seq (.havoc "Y") (.havoc "X")
+    private def copy: Command := .seq (.havoc "X") (.assign "Y" "X")
+    private def whileHavoc: Command :=
+      .while (.not (.eq "X" 0))
+        (.seq (.havoc "X") (.assign "X" ("X" + 1)))
+    private def whileSkip: Command := .while (.not (.eq "X" 0)) .skip
+    private def havocHavoc: Command :=
+      .while (.neq "X" 0)
+        (.seq (.havoc "X") (.havoc "Y"))
+    private def noHavoc: Command := .seq (.assign "X" 0) (.assign "Z" 1)
+
+    namespace Term
+      example: CommandEval (.havoc "X") State.empty (State.build [("X", 0)]) := sorry
+      example: CommandEval (.seq .skip (.havoc "Z")) State.empty (State.build [("Z", 42)]) := sorry
+
+      example: xy.equiv yx ∨ ¬(xy.equiv yx) := sorry
+      example: xy.equiv copy ∨ ¬(xy.equiv copy) := sorry
+
+      theorem whileHavoc.may_diverge (s₁ s₂: State) (h: s₁ "X" ≠ 0): ¬(CommandEval whileHavoc s₁ s₂) := sorry
+      theorem whileSkip.may_diverge (s₁ s₂: State) (h: s₁ "X" ≠ 0): ¬(CommandEval whileSkip s₁ s₂) := sorry
+      example: whileHavoc.equiv whileSkip := sorry
+
+      example: ¬(havocHavoc.equiv noHavoc) := sorry
+
+      example: (Command.while (.neq "X" 1) (.havoc "X")).equiv (.assign "X" 1) := sorry
+    end Term
+
+    namespace Tactic
+      example: CommandEval (.havoc "X") State.empty (State.build [("X", 0)]) := by sorry
+      example: CommandEval (.seq .skip (.havoc "Z")) State.empty (State.build [("Z", 42)]) := by sorry
+
+      example: xy.equiv yx ∨ ¬(xy.equiv yx) := by sorry
+      example: xy.equiv copy ∨ ¬(xy.equiv copy) := by sorry
+
+      theorem whileHavoc.may_diverge (s₁ s₂: State) (h: s₁ "X" ≠ 0): ¬(CommandEval whileHavoc s₁ s₂) := by sorry
+      theorem whileSkip.may_diverge (s₁ s₂: State) (h: s₁ "X" ≠ 0): ¬(CommandEval whileSkip s₁ s₂) := by sorry
+      example: whileHavoc.equiv whileSkip := by sorry
+
+      example: ¬(havocHavoc.equiv noHavoc) := by sorry
+
+      example: (Command.while (.neq "X" 1) (.havoc "X")).equiv (.assign "X" 1) := by sorry
+    end Tactic
+
+    namespace Blended
+      example: CommandEval (.havoc "X") State.empty (State.build [("X", 0)]) := sorry
+      example: CommandEval (.seq .skip (.havoc "Z")) State.empty (State.build [("Z", 42)]) := sorry
+
+      example: xy.equiv yx ∨ ¬(xy.equiv yx) := sorry
+      example: xy.equiv copy ∨ ¬(xy.equiv copy) := sorry
+
+      theorem whileHavoc.may_diverge (s₁ s₂: State) (h: s₁ "X" ≠ 0): ¬(CommandEval whileHavoc s₁ s₂) := sorry
+      theorem whileSkip.may_diverge (s₁ s₂: State) (h: s₁ "X" ≠ 0): ¬(CommandEval whileSkip s₁ s₂) := sorry
+      example: whileHavoc.equiv whileSkip := sorry
+
+      example: ¬(havocHavoc.equiv noHavoc) := sorry
+
+      example: (Command.while (.neq "X" 1) (.havoc "X")).equiv (.assign "X" 1) := sorry
+    end Blended
+  end Havoc
+
+  /-
+  ## Additional Exercises
+  -/
+
+  -- How is this different from "refines" above?
+  @[reducible] def _root_.Command.approx  (c₁ c₂: Command): Prop := ∀ s₁ s₂: State, CommandEval c₁ s₁ s₂ → CommandEval c₂ s₁ s₂
+
+  private def approx_c₁: Command := .while (.neq "X" 1) (.assign "X" ("X" - 1))
+  private def approx_c₂: Command := .assign "X" 1
+
+  private def approx_c₃: Command := sorry
+  private def approx_c₄: Command := sorry
+
+  private def approx_min: Command := sorry
+
+  private def _root_.Command.zProp (c: Command): Prop := sorry
+
+  namespace Term
+    example (id₁ id₂: String) (e₁ e₂: Arith) (h₁: OccursCheck id₁ e₁) (h₂: OccursCheck id₂ e₂): (Command.seq (.assign id₁ e₁) (.assign id₂ e₂)).equiv (.seq (.assign id₂ e₂) (.assign id₁ e₁)) := sorry
+
+    -- TODO: For loops in Imp
+
+    example: ¬(approx_c₃.approx approx_c₄) ∧ ¬(approx_c₄.approx approx_c₃) := sorry
+    example (c: Command): approx_min.approx c := sorry
+    example (c₁ c₂: Command) (h₁: c₁.zProp) (h₂: c₁.approx c₂): c₂.zProp := sorry
+  end Term
+
+  namespace Tactic
+    example (id₁ id₂: String) (e₁ e₂: Arith) (h₁: OccursCheck id₁ e₁) (h₂: OccursCheck id₂ e₂): (Command.seq (.assign id₁ e₁) (.assign id₂ e₂)).equiv (.seq (.assign id₂ e₂) (.assign id₁ e₁)) := by sorry
+
+    -- TODO: For loops in Imp
+
+    example: ¬(approx_c₃.approx approx_c₄) ∧ ¬(approx_c₄.approx approx_c₃) := by sorry
+    example (c: Command): approx_min.approx c := by sorry
+    example (c₁ c₂: Command) (h₁: c₁.zProp) (h₂: c₁.approx c₂): c₂.zProp := by sorry
+  end Tactic
+
+  namespace Blended
+    example (id₁ id₂: String) (e₁ e₂: Arith) (h₁: OccursCheck id₁ e₁) (h₂: OccursCheck id₂ e₂): (Command.seq (.assign id₁ e₁) (.assign id₂ e₂)).equiv (.seq (.assign id₂ e₂) (.assign id₁ e₁)) := sorry
+
+    -- TODO: For loops in Imp
+
+    example: ¬(approx_c₃.approx approx_c₄) ∧ ¬(approx_c₄.approx approx_c₃) := sorry
+    example (c: Command): approx_min.approx c := sorry
+    example (c₁ c₂: Command) (h₁: c₁.zProp) (h₂: c₁.approx c₂): c₂.zProp := sorry
+  end Blended
+end SoftwareFoundations.ProgrammingLanguageFoundations.Equiv
